arm-hyp execspec: add irqVGICMaintenane and initInterruptController
with caseconvs, generated files

spec/design/ARM_HYP/ArchStructures_H.thy
@@ -188,6 +188,232 @@ where
 datatype asidpool =
     ASIDPool "asid \<Rightarrow> ((machine_word) option)"
 
+type_synonym virq = "machine_word"
+
+datatype gicvcpuinterface =
+    VGICInterface machine_word machine_word machine_word "nat \<Rightarrow> virq"
+
+primrec
+  vgicLR :: "gicvcpuinterface \<Rightarrow> nat \<Rightarrow> virq"
+where
+  "vgicLR (VGICInterface v0 v1 v2 v3) = v3"
+
+primrec
+  vgicHCR :: "gicvcpuinterface \<Rightarrow> machine_word"
+where
+  "vgicHCR (VGICInterface v0 v1 v2 v3) = v0"
+
+primrec
+  vgicVMCR :: "gicvcpuinterface \<Rightarrow> machine_word"
+where
+  "vgicVMCR (VGICInterface v0 v1 v2 v3) = v1"
+
+primrec
+  vgicAPR :: "gicvcpuinterface \<Rightarrow> machine_word"
+where
+  "vgicAPR (VGICInterface v0 v1 v2 v3) = v2"
+
+primrec
+  vgicLR_update :: "((nat \<Rightarrow> virq) \<Rightarrow> (nat \<Rightarrow> virq)) \<Rightarrow> gicvcpuinterface \<Rightarrow> gicvcpuinterface"
+where
+  "vgicLR_update f (VGICInterface v0 v1 v2 v3) = VGICInterface v0 v1 v2 (f v3)"
+
+primrec
+  vgicHCR_update :: "(machine_word \<Rightarrow> machine_word) \<Rightarrow> gicvcpuinterface \<Rightarrow> gicvcpuinterface"
+where
+  "vgicHCR_update f (VGICInterface v0 v1 v2 v3) = VGICInterface (f v0) v1 v2 v3"
+
+primrec
+  vgicVMCR_update :: "(machine_word \<Rightarrow> machine_word) \<Rightarrow> gicvcpuinterface \<Rightarrow> gicvcpuinterface"
+where
+  "vgicVMCR_update f (VGICInterface v0 v1 v2 v3) = VGICInterface v0 (f v1) v2 v3"
+
+primrec
+  vgicAPR_update :: "(machine_word \<Rightarrow> machine_word) \<Rightarrow> gicvcpuinterface \<Rightarrow> gicvcpuinterface"
+where
+  "vgicAPR_update f (VGICInterface v0 v1 v2 v3) = VGICInterface v0 v1 (f v2) v3"
+
+abbreviation (input)
+  VGICInterface_trans :: "(machine_word) \<Rightarrow> (machine_word) \<Rightarrow> (machine_word) \<Rightarrow> (nat \<Rightarrow> virq) \<Rightarrow> gicvcpuinterface" ("VGICInterface'_ \<lparr> vgicHCR= _, vgicVMCR= _, vgicAPR= _, vgicLR= _ \<rparr>")
+where
+  "VGICInterface_ \<lparr> vgicHCR= v0, vgicVMCR= v1, vgicAPR= v2, vgicLR= v3 \<rparr> == VGICInterface v0 v1 v2 v3"
+
+lemma vgicLR_vgicLR_update [simp]:
+  "vgicLR (vgicLR_update f v) = f (vgicLR v)"
+  by (cases v) simp
+
+lemma vgicLR_vgicHCR_update [simp]:
+  "vgicLR (vgicHCR_update f v) = vgicLR v"
+  by (cases v) simp
+
+lemma vgicLR_vgicVMCR_update [simp]:
+  "vgicLR (vgicVMCR_update f v) = vgicLR v"
+  by (cases v) simp
+
+lemma vgicLR_vgicAPR_update [simp]:
+  "vgicLR (vgicAPR_update f v) = vgicLR v"
+  by (cases v) simp
+
+lemma vgicHCR_vgicLR_update [simp]:
+  "vgicHCR (vgicLR_update f v) = vgicHCR v"
+  by (cases v) simp
+
+lemma vgicHCR_vgicHCR_update [simp]:
+  "vgicHCR (vgicHCR_update f v) = f (vgicHCR v)"
+  by (cases v) simp
+
+lemma vgicHCR_vgicVMCR_update [simp]:
+  "vgicHCR (vgicVMCR_update f v) = vgicHCR v"
+  by (cases v) simp
+
+lemma vgicHCR_vgicAPR_update [simp]:
+  "vgicHCR (vgicAPR_update f v) = vgicHCR v"
+  by (cases v) simp
+
+lemma vgicVMCR_vgicLR_update [simp]:
+  "vgicVMCR (vgicLR_update f v) = vgicVMCR v"
+  by (cases v) simp
+
+lemma vgicVMCR_vgicHCR_update [simp]:
+  "vgicVMCR (vgicHCR_update f v) = vgicVMCR v"
+  by (cases v) simp
+
+lemma vgicVMCR_vgicVMCR_update [simp]:
+  "vgicVMCR (vgicVMCR_update f v) = f (vgicVMCR v)"
+  by (cases v) simp
+
+lemma vgicVMCR_vgicAPR_update [simp]:
+  "vgicVMCR (vgicAPR_update f v) = vgicVMCR v"
+  by (cases v) simp
+
+lemma vgicAPR_vgicLR_update [simp]:
+  "vgicAPR (vgicLR_update f v) = vgicAPR v"
+  by (cases v) simp
+
+lemma vgicAPR_vgicHCR_update [simp]:
+  "vgicAPR (vgicHCR_update f v) = vgicAPR v"
+  by (cases v) simp
+
+lemma vgicAPR_vgicVMCR_update [simp]:
+  "vgicAPR (vgicVMCR_update f v) = vgicAPR v"
+  by (cases v) simp
+
+lemma vgicAPR_vgicAPR_update [simp]:
+  "vgicAPR (vgicAPR_update f v) = f (vgicAPR v)"
+  by (cases v) simp
+
+datatype vcpu =
+    VCPUObj "(machine_word) option" machine_word machine_word gicvcpuinterface
+
+primrec
+  vcpuSCTLR :: "vcpu \<Rightarrow> machine_word"
+where
+  "vcpuSCTLR (VCPUObj v0 v1 v2 v3) = v1"
+
+primrec
+  vcpuVGIC :: "vcpu \<Rightarrow> gicvcpuinterface"
+where
+  "vcpuVGIC (VCPUObj v0 v1 v2 v3) = v3"
+
+primrec
+  vcpuTCBPtr :: "vcpu \<Rightarrow> (machine_word) option"
+where
+  "vcpuTCBPtr (VCPUObj v0 v1 v2 v3) = v0"
+
+primrec
+  vcpuACTLR :: "vcpu \<Rightarrow> machine_word"
+where
+  "vcpuACTLR (VCPUObj v0 v1 v2 v3) = v2"
+
+primrec
+  vcpuSCTLR_update :: "(machine_word \<Rightarrow> machine_word) \<Rightarrow> vcpu \<Rightarrow> vcpu"
+where
+  "vcpuSCTLR_update f (VCPUObj v0 v1 v2 v3) = VCPUObj v0 (f v1) v2 v3"
+
+primrec
+  vcpuVGIC_update :: "(gicvcpuinterface \<Rightarrow> gicvcpuinterface) \<Rightarrow> vcpu \<Rightarrow> vcpu"
+where
+  "vcpuVGIC_update f (VCPUObj v0 v1 v2 v3) = VCPUObj v0 v1 v2 (f v3)"
+
+primrec
+  vcpuTCBPtr_update :: "(((machine_word) option) \<Rightarrow> ((machine_word) option)) \<Rightarrow> vcpu \<Rightarrow> vcpu"
+where
+  "vcpuTCBPtr_update f (VCPUObj v0 v1 v2 v3) = VCPUObj (f v0) v1 v2 v3"
+
+primrec
+  vcpuACTLR_update :: "(machine_word \<Rightarrow> machine_word) \<Rightarrow> vcpu \<Rightarrow> vcpu"
+where
+  "vcpuACTLR_update f (VCPUObj v0 v1 v2 v3) = VCPUObj v0 v1 (f v2) v3"
+
+abbreviation (input)
+  VCPUObj_trans :: "((machine_word) option) \<Rightarrow> (machine_word) \<Rightarrow> (machine_word) \<Rightarrow> (gicvcpuinterface) \<Rightarrow> vcpu" ("VCPUObj'_ \<lparr> vcpuTCBPtr= _, vcpuSCTLR= _, vcpuACTLR= _, vcpuVGIC= _ \<rparr>")
+where
+  "VCPUObj_ \<lparr> vcpuTCBPtr= v0, vcpuSCTLR= v1, vcpuACTLR= v2, vcpuVGIC= v3 \<rparr> == VCPUObj v0 v1 v2 v3"
+
+lemma vcpuSCTLR_vcpuSCTLR_update [simp]:
+  "vcpuSCTLR (vcpuSCTLR_update f v) = f (vcpuSCTLR v)"
+  by (cases v) simp
+
+lemma vcpuSCTLR_vcpuVGIC_update [simp]:
+  "vcpuSCTLR (vcpuVGIC_update f v) = vcpuSCTLR v"
+  by (cases v) simp
+
+lemma vcpuSCTLR_vcpuTCBPtr_update [simp]:
+  "vcpuSCTLR (vcpuTCBPtr_update f v) = vcpuSCTLR v"
+  by (cases v) simp
+
+lemma vcpuSCTLR_vcpuACTLR_update [simp]:
+  "vcpuSCTLR (vcpuACTLR_update f v) = vcpuSCTLR v"
+  by (cases v) simp
+
+lemma vcpuVGIC_vcpuSCTLR_update [simp]:
+  "vcpuVGIC (vcpuSCTLR_update f v) = vcpuVGIC v"
+  by (cases v) simp
+
+lemma vcpuVGIC_vcpuVGIC_update [simp]:
+  "vcpuVGIC (vcpuVGIC_update f v) = f (vcpuVGIC v)"
+  by (cases v) simp
+
+lemma vcpuVGIC_vcpuTCBPtr_update [simp]:
+  "vcpuVGIC (vcpuTCBPtr_update f v) = vcpuVGIC v"
+  by (cases v) simp
+
+lemma vcpuVGIC_vcpuACTLR_update [simp]:
+  "vcpuVGIC (vcpuACTLR_update f v) = vcpuVGIC v"
+  by (cases v) simp
+
+lemma vcpuTCBPtr_vcpuSCTLR_update [simp]:
+  "vcpuTCBPtr (vcpuSCTLR_update f v) = vcpuTCBPtr v"
+  by (cases v) simp
+
+lemma vcpuTCBPtr_vcpuVGIC_update [simp]:
+  "vcpuTCBPtr (vcpuVGIC_update f v) = vcpuTCBPtr v"
+  by (cases v) simp
+
+lemma vcpuTCBPtr_vcpuTCBPtr_update [simp]:
+  "vcpuTCBPtr (vcpuTCBPtr_update f v) = f (vcpuTCBPtr v)"
+  by (cases v) simp
+
+lemma vcpuTCBPtr_vcpuACTLR_update [simp]:
+  "vcpuTCBPtr (vcpuACTLR_update f v) = vcpuTCBPtr v"
+  by (cases v) simp
+
+lemma vcpuACTLR_vcpuSCTLR_update [simp]:
+  "vcpuACTLR (vcpuSCTLR_update f v) = vcpuACTLR v"
+  by (cases v) simp
+
+lemma vcpuACTLR_vcpuVGIC_update [simp]:
+  "vcpuACTLR (vcpuVGIC_update f v) = vcpuACTLR v"
+  by (cases v) simp
+
+lemma vcpuACTLR_vcpuTCBPtr_update [simp]:
+  "vcpuACTLR (vcpuTCBPtr_update f v) = vcpuACTLR v"
+  by (cases v) simp
+
+lemma vcpuACTLR_vcpuACTLR_update [simp]:
+  "vcpuACTLR (vcpuACTLR_update f v) = f (vcpuACTLR v)"
+  by (cases v) simp
+
 datatype arch_kernel_object =
     KOASIDPool asidpool
   | KOPTE pte
@@ -211,6 +437,9 @@ asidRange :: "(asid * asid)"
 consts'
 asidHighBitsOf :: "asid \<Rightarrow> asid"
 
+consts'
+makeVCPUObject :: "vcpu"
+
 defs archObjSize_def:
 "archObjSize a\<equiv> (case a of
                   KOASIDPool v10 \<Rightarrow>   pageBits
@@ -232,6 +461,39 @@ defs asidRange_def:
 
 defs asidHighBitsOf_def:
 "asidHighBitsOf asid\<equiv> (asid `~shiftR~` asidLowBits) && mask asidHighBits"
+
+definition
+"gicVCPUMaxNumLR\<equiv> (64 ::nat)"
+
+definition
+"hcrVCPU\<equiv>  (0x87039 ::machine_word)"
+
+definition
+"hcrNative\<equiv> (0xfe8703b ::machine_word)"
+
+definition
+"vgicHCREN\<equiv> (0x1 ::machine_word)"
+
+definition
+"sctlrDefault\<equiv> (0xc5187c ::machine_word)"
+
+definition
+"actlrDefault\<equiv> (0x40 ::machine_word)"
+
+defs makeVCPUObject_def:
+"makeVCPUObject \<equiv>
+    let vgicLR = funPartialArray (const (0 ::machine_word)) (0, gicVCPUMaxNumLR- 1) in
+    VCPUObj_ \<lparr>
+          vcpuTCBPtr= Nothing
+        , vcpuSCTLR= sctlrDefault
+        , vcpuACTLR= actlrDefault
+        , vcpuVGIC= VGICInterface_ \<lparr>
+                          vgicHCR= vgicHCREN
+                        , vgicVMCR= 0
+                        , vgicAPR= 0
+                        , vgicLR= vgicLR
+                        \<rparr>
+        \<rparr>"
 
 
 datatype arch_kernel_object_type =
