spec/design/ARM_HYP/ArchHypervisor_H.thy
@@ -1,0 +1,188 @@
+(*
+ * Copyright 2014, General Dynamics C4 Systems
+ *
+ * This software may be distributed and modified according to the terms of
+ * the GNU General Public License version 2. Note that NO WARRANTY is provided.
+ * See "LICENSE_GPLv2.txt" for details.
+ *
+ * @TAG(GD_GPL)
+ *)
+
+(* 
+  VSpace lookup code.
+*)
+
+theory ArchHypervisor_H
+imports
+  "../CNode_H"
+(*  "../KI_Decls_H"
+  ArchVSpaceDecls_H *)
+begin
+context Arch begin global_naming ARM_HYP_H
+
+
+consts'
+handleHypervisorFault :: "machine_word \<Rightarrow> hyp_fault_type \<Rightarrow> unit kernel"
+
+
+defs handleHypervisorFault_def:
+"handleHypervisorFault arg1 hyp \<equiv> case hyp of ARMNoHypFaults \<Rightarrow> haskell_fail []"
+
+definition
+vcpuEnable :: "machine_word \<Rightarrow> unit kernel"
+where
+"vcpuEnable vcpuPtr\<equiv> (do
+    vcpu \<leftarrow> getObject vcpuPtr;
+    doMachineOp $ (do
+        setSCTLR (vcpuSCTLR vcpu);
+        setHCR hcrVCPU;
+        isb;
+        set_gic_vcpu_ctrl_hcr (vgicHCR \<circ> vcpuVGIC $ vcpu)
+    od)
+od)"
+
+definition
+vcpuDisable :: "(machine_word) option \<Rightarrow> unit kernel"
+where
+"vcpuDisable vcpuPtrOpt\<equiv> (do
+    doMachineOp dsb;
+    (case vcpuPtrOpt of
+          Some vcpuPtr \<Rightarrow>   (do
+           vcpu \<leftarrow> getObject vcpuPtr;
+           hcr \<leftarrow> doMachineOp get_gic_vcpu_ctrl_hcr;
+           sctlr \<leftarrow> doMachineOp getSCTLR;
+           setObject vcpuPtr $ vcpu \<lparr>
+                 vcpuSCTLR := sctlr
+               , vcpuVGIC := (vcpuVGIC vcpu) \<lparr> vgicHCR := hcr \<rparr>
+               \<rparr>
+          od)
+        | None \<Rightarrow>   return ()
+        );
+    doMachineOp $ (do
+        set_gic_vcpu_ctrl_hcr 0;
+        isb;
+        setSCTLR sctlrDefault;
+        setHCR hcrNative;
+        isb
+    od)
+od)"
+
+definition
+vcpuSave :: "(machine_word * bool) option \<Rightarrow> unit kernel"
+where
+"vcpuSave x0\<equiv> (case x0 of
+    (Some (vcpuPtr, active)) \<Rightarrow>    (do
+    doMachineOp dsb;
+    vcpu \<leftarrow> getObject vcpuPtr;
+    (hcr, sctlr) \<leftarrow> if active
+                        then (do
+                            sctlr \<leftarrow> doMachineOp getSCTLR;
+                            hcr \<leftarrow> doMachineOp get_gic_vcpu_ctrl_hcr;
+                            return (sctlr, hcr)
+                        od)
+                        else return (vcpuSCTLR vcpu, vgicHCR \<circ> vcpuVGIC $ vcpu);
+    actlr \<leftarrow> doMachineOp getACTLR;
+    vmcr \<leftarrow> doMachineOp get_gic_vcpu_ctrl_vmcr;
+    apr \<leftarrow> doMachineOp get_gic_vcpu_ctrl_apr;
+    numListRegs \<leftarrow> gets (armKSGICVCPUNumListRegs \<circ> ksArchState);
+    gicIndices \<leftarrow> return ( [0 .e. numListRegs- 1]);
+    lrVals \<leftarrow> doMachineOp $ mapM get_gic_vcpu_ctrl_lr gicIndices;
+    vcpuLR \<leftarrow> return ( (vgicLR \<circ> vcpuVGIC $ vcpu)  aLU  zip gicIndices lrVals);
+    setObject vcpuPtr $ vcpu \<lparr>
+          vcpuSCTLR := sctlr
+        , vcpuACTLR := actlr
+        , vcpuVGIC := (vcpuVGIC vcpu) \<lparr> vgicHCR := hcr
+                                     , vgicVMCR := vmcr
+                                     , vgicAPR := apr
+                                     , vgicLR := vcpuLR \<rparr>
+        \<rparr>;
+    doMachineOp isb
+    od)
+  | _ \<Rightarrow>    haskell_fail []
+  )"
+
+definition
+vcpuRestore :: "machine_word \<Rightarrow> unit kernel"
+where
+"vcpuRestore vcpuPtr\<equiv> (do
+    doMachineOp $ set_gic_vcpu_ctrl_hcr 0;
+    doMachineOp $ isb;
+    vcpu \<leftarrow> getObject vcpuPtr;
+    vgic \<leftarrow> return ( vcpuVGIC vcpu);
+    doMachineOp $ (do
+        set_gic_vcpu_ctrl_vmcr (vgicVMCR vgic);
+        set_gic_vcpu_ctrl_apr (vgicAPR vgic);
+        mapM_x (uncurry set_gic_vcpu_ctrl_lr) (map (\<lambda> i. (i, (vgicLR vgic) i)) [0 .e. gicVCPUMaxNumLR- 1]);
+        setACTLR (vcpuACTLR vcpu)
+    od);
+    vcpuEnable vcpuPtr
+od)"
+
+definition
+vcpuInvalidateActive :: "unit kernel"
+where
+"vcpuInvalidateActive\<equiv> (do
+    hsCurVCPU \<leftarrow> gets (armHSCurVCPU \<circ> ksArchState);
+    (case hsCurVCPU of
+          Some (vcpuPtr, True) \<Rightarrow>   (do
+            vcpuDisable Nothing;
+            modifyArchState (\<lambda> s. s \<lparr> armHSCurVCPU := Just (vcpuPtr, False) \<rparr>)
+          od)
+        | _ \<Rightarrow>   return ()
+        )
+od)"
+
+definition
+"vcpuCleanInvalidateActive\<equiv> (do
+    hsCurVCPU \<leftarrow> gets (armHSCurVCPU \<circ> ksArchState);
+    vcpuSave hsCurVCPU;
+    vcpuInvalidateActive
+od)"
+
+definition
+vcpuSwitch :: "(machine_word) option \<Rightarrow> unit kernel"
+where
+"vcpuSwitch x0\<equiv> (case x0 of
+    None \<Rightarrow>    (do
+    hsCurVCPU \<leftarrow> gets (armHSCurVCPU \<circ> ksArchState);
+    (case hsCurVCPU of
+          None \<Rightarrow>   return ()
+        | Some (vcpuPtr, active) \<Rightarrow>   (do
+            when active $ (do
+                vcpuDisable (Just vcpuPtr);
+                modifyArchState (\<lambda> s. s \<lparr> armHSCurVCPU := Just (vcpuPtr, False) \<rparr>)
+            od);
+            return ()
+        od)
+        )
+    od)
+  | (Some new) \<Rightarrow>    (do
+    hsCurVCPU \<leftarrow> gets (armHSCurVCPU \<circ> ksArchState);
+    (case hsCurVCPU of
+          None \<Rightarrow>   (do
+            vcpuRestore new;
+            modifyArchState (\<lambda> s. s \<lparr> armHSCurVCPU := Just (new, True) \<rparr>)
+          od)
+        | Some (vcpuPtr, active) \<Rightarrow>   (
+            if vcpuPtr \<noteq> new
+                then (do
+                    vcpuSave hsCurVCPU;
+                    vcpuRestore new;
+                    modifyArchState (\<lambda> s. s \<lparr> armHSCurVCPU := Just (new, True) \<rparr>)
+                od)
+                else (
+                    when (Not active) $ (do
+                        doMachineOp isb;
+                        vcpuEnable new;
+                        modifyArchState (\<lambda> s. s \<lparr> armHSCurVCPU := Just (new, False) \<rparr>)
+                    od)
+                )
+        )
+        )
+  od)
+  )"
+
+
+
+end
+end
