spec/design/ARM_HYP/ArchVSpaceDecls_H.thy
@@ -217,6 +217,9 @@ consts'
 resolveVAddr :: "machine_word \<Rightarrow> vptr \<Rightarrow> ((vmpage_size * paddr) option) kernel"
 
 consts'
+isIOSpaceFrameCap :: "arch_capability \<Rightarrow> bool"
+
+consts'
 decodeARMMMUInvocation :: "machine_word \<Rightarrow> machine_word list \<Rightarrow> cptr \<Rightarrow> machine_word \<Rightarrow> arch_capability \<Rightarrow> (capability * machine_word) list \<Rightarrow> ( syscall_error , invocation ) kernel_f"
 
 consts'
