spec/design/ARM_HYP/VCPU_H.thy
@@ -1,0 +1,263 @@
+(*
+ * Copyright 2014, General Dynamics C4 Systems
+ *
+ * This software may be distributed and modified according to the terms of
+ * the GNU General Public License version 2. Note that NO WARRANTY is provided.
+ * See "LICENSE_GPLv2.txt" for details.
+ *
+ * @TAG(GD_GPL)
+ *)
+
+chapter "VCPU"
+
+theory VCPU_H
+imports Hardware_H "../Structures_H"
+  "../Invocations_H"
+  "../TCB_H"
+begin
+context Arch begin global_naming ARM_HYP_H
+
+definition
+decodeVCPUSetTCB :: "arch_capability \<Rightarrow> (capability * machine_word) list \<Rightarrow> ( syscall_error , Arch.invocation ) kernel_f"
+where
+"decodeVCPUSetTCB x0 extraCaps\<equiv> (let cap = x0 in
+  if isVCPUCap cap then   (doE
+    whenE (null extraCaps) $ throw TruncatedMessage;
+    tcbPtr \<leftarrow> (case fst (head extraCaps) of
+          ThreadCap tcbPtr \<Rightarrow>   returnOk tcbPtr
+        | _ \<Rightarrow>   throw IllegalOperation
+        );
+    returnOk $ InvokeVCPU $ VCPUSetTCB (capVCPUPtr cap) tcbPtr
+  odE)
+  else   throw IllegalOperation
+  )"
+
+definition
+dissociateVCPUTCB :: "machine_word \<Rightarrow> machine_word \<Rightarrow> unit kernel"
+where
+"dissociateVCPUTCB vcpuPtr tcbPtr\<equiv> (do
+    tcbVCPU \<leftarrow> archThreadGet atcbVCPUPtr tcbPtr;
+    vcpu \<leftarrow> getObject vcpuPtr;
+    vcpuTCB \<leftarrow> return ( vcpuTCBPtr vcpu);
+    when (tcbVCPU \<noteq> Just vcpuPtr \<or> vcpuTCB \<noteq> Just tcbPtr) $
+        haskell_fail [];
+    setObject vcpuPtr $ vcpu \<lparr> vcpuTCBPtr := Nothing \<rparr>;
+    archThreadSet (\<lambda> atcb. atcb \<lparr> atcbVCPUPtr := Nothing \<rparr>) tcbPtr
+od)"
+
+definition
+associateVCPUTCB :: "machine_word \<Rightarrow> machine_word \<Rightarrow> unit kernel"
+where
+"associateVCPUTCB vcpuPtr tcbPtr\<equiv> (do
+    tcbVCPU \<leftarrow> archThreadGet atcbVCPUPtr tcbPtr;
+    (case tcbVCPU of
+        Some ptr \<Rightarrow>   dissociateVCPUTCB ptr tcbPtr
+      | _ \<Rightarrow>   return ()
+      );
+    vcpu \<leftarrow> getObject vcpuPtr;
+    (case (vcpuTCBPtr vcpu) of
+          Some ptr \<Rightarrow>   dissociateVCPUTCB vcpuPtr ptr
+        | _ \<Rightarrow>   return ()
+        );
+    archThreadSet (\<lambda> atcb. atcb \<lparr> atcbVCPUPtr := Just vcpuPtr \<rparr>) tcbPtr;
+    setObject vcpuPtr $ vcpu \<lparr> vcpuTCBPtr := Just tcbPtr \<rparr>
+od)"
+
+definition
+decodeVCPUReadReg :: "machine_word list \<Rightarrow> arch_capability \<Rightarrow> ( syscall_error , Arch.invocation ) kernel_f"
+where
+"decodeVCPUReadReg x0 x1\<equiv> (let (ls, cap) = (x0, x1) in
+  if isVCPUCap cap \<and> length ls > 0
+  then let field = ls ! 0 in   (doE
+    whenE (field \<noteq> 0) $ throw (InvalidArgument 1);
+    returnOk $ InvokeVCPU $
+        VCPUReadRegister (capVCPUPtr cap) (fromIntegral field)
+  odE)
+  else   throw TruncatedMessage
+  )"
+
+definition
+decodeVCPUWriteReg :: "machine_word list \<Rightarrow> arch_capability \<Rightarrow> ( syscall_error , Arch.invocation ) kernel_f"
+where
+"decodeVCPUWriteReg x0 x1\<equiv> (let (ls, cap) = (x0, x1) in
+  if isVCPUCap cap \<and> length ls > 1
+  then let field = ls ! 0; val = ls ! 1
+  in   (doE
+    whenE (field \<noteq> 0) $ throw (InvalidArgument 1);
+    returnOk $ InvokeVCPU $ VCPUWriteRegister (capVCPUPtr cap)
+                (fromIntegral field) (fromIntegral val)
+  odE)
+  else   throw TruncatedMessage
+  )"
+
+definition
+readVCPUReg :: "machine_word \<Rightarrow> hyper_reg \<Rightarrow> hyper_reg_val kernel"
+where
+"readVCPUReg vcpuPtr reg\<equiv> (
+    if reg = 0
+        then (do
+            vcpu \<leftarrow> getObject vcpuPtr;
+            return $ vcpuSCTLR vcpu
+        od)
+        else haskell_fail []
+)"
+
+definition
+writeVCPUReg :: "machine_word \<Rightarrow> hyper_reg \<Rightarrow> hyper_reg_val \<Rightarrow> unit kernel"
+where
+"writeVCPUReg vcpuPtr reg val \<equiv>
+    if reg = 0
+        then (do
+            vcpu \<leftarrow> getObject vcpuPtr;
+            setObject vcpuPtr $ vcpu \<lparr> vcpuSCTLR := val \<rparr>
+        od)
+        else haskell_fail []"
+
+definition
+invokeVCPUReadReg :: "machine_word \<Rightarrow> hyper_reg \<Rightarrow> unit kernel"
+where
+"invokeVCPUReadReg vcpuPtr reg\<equiv> (do
+    ct \<leftarrow> getCurThread;
+    hsCurVCPU \<leftarrow> gets (armHSCurVCPU \<circ> ksArchState);
+    (case hsCurVCPU of
+          Some (vcpuPtr, _) \<Rightarrow>  
+           vcpuCleanInvalidateActive
+        | _ \<Rightarrow>   return ()
+        );
+    val \<leftarrow> readVCPUReg vcpuPtr reg;
+    asUser ct $ setRegister (msgRegisters ! 0) $ fromIntegral val;
+    msgInfo \<leftarrow> return ( MI_ \<lparr>
+            msgLength= 1,
+            msgExtraCaps= 0,
+            msgCapsUnwrapped= 0,
+            msgLabel= 0 \<rparr>);
+    setMessageInfo ct msgInfo;
+    setThreadState Running ct
+od)"
+
+definition
+invokeVCPUWriteReg :: "machine_word \<Rightarrow> hyper_reg \<Rightarrow> hyper_reg_val \<Rightarrow> unit kernel"
+where
+"invokeVCPUWriteReg vcpuPtr reg val\<equiv> (do
+    hsCurVCPU \<leftarrow> gets (armHSCurVCPU \<circ> ksArchState);
+    (case hsCurVCPU of
+          Some (vcpuPtr, _) \<Rightarrow>  
+            vcpuCleanInvalidateActive
+        | _ \<Rightarrow>   return ()
+        );
+    writeVCPUReg vcpuPtr reg val;
+    ct \<leftarrow> getCurThread;
+    setThreadState Restart ct
+od)"
+
+definition
+makeVIRQ :: "machine_word \<Rightarrow> machine_word \<Rightarrow> machine_word \<Rightarrow> virq"
+where
+"makeVIRQ group prio irq \<equiv>
+    let
+     groupShift = 30;
+          prioShift = 23;
+          irqPending = bit 28;
+          eoiirqen = bit 19
+    in
+    (group `~shiftL~` groupShift) || (prio `~shiftL~` prioShift) || irq ||
+        irqPending || eoiirqen"
+
+definition
+decodeVCPUInjectIRQ :: "machine_word list \<Rightarrow> arch_capability \<Rightarrow> ( syscall_error , Arch.invocation ) kernel_f"
+where
+"decodeVCPUInjectIRQ x0 x1\<equiv> (let (ls, cap) = (x0, x1) in
+  if isVCPUCap cap \<and> length ls > 1
+  then let mr0 = ls ! 0; mr1 = ls ! 1
+  in   (doE
+    vcpuPtr \<leftarrow> returnOk ( capVCPUPtr cap);
+    vid \<leftarrow> returnOk ( mr0 && 0xffff);
+    priority \<leftarrow> returnOk ( (mr0 `~shiftR~` 16) && 0xff);
+    group \<leftarrow> returnOk ( (mr0 `~shiftR~` 24) && 0xff);
+    index \<leftarrow> returnOk ( mr1 && 0xff);
+    rangeCheck vid (0::nat) ((1 `~shiftL~` 10) - 1);
+    rangeCheck priority (0::nat) 31;
+    rangeCheck group (0::nat) 1;
+    gic_vcpu_num_list_regs \<leftarrow> withoutFailure $
+        gets (armKSGICVCPUNumListRegs \<circ> ksArchState);
+    rangeCheck index 0 gic_vcpu_num_list_regs;
+    vcpuLR \<leftarrow> withoutFailure $ liftM (vgicLR \<circ> vcpuVGIC) $ getObject vcpuPtr;
+    whenE (vcpuLR (fromIntegral index) && vgicIRQMask = vgicIRQActive) $
+        throw DeleteFirst;
+    virq \<leftarrow> returnOk ( makeVIRQ (fromIntegral group) (fromIntegral priority) (fromIntegral vid));
+    returnOk $ InvokeVCPU $ VCPUInjectIRQ vcpuPtr (fromIntegral index) virq
+  odE)
+  else   throw TruncatedMessage
+  )"
+
+definition
+invokeVCPUInjectIRQ :: "machine_word \<Rightarrow> nat \<Rightarrow> virq \<Rightarrow> unit kernel"
+where
+"invokeVCPUInjectIRQ vcpuPtr index virq\<equiv> (do
+    hsCurVCPU \<leftarrow> gets (armHSCurVCPU \<circ> ksArchState);
+    (case hsCurVCPU of
+          Some (vcpuPtr, _) \<Rightarrow>  
+            doMachineOp $ set_gic_vcpu_ctrl_lr index virq
+        | _ \<Rightarrow>   (do
+             vcpu \<leftarrow> getObject vcpuPtr;
+             vcpuLR \<leftarrow> return ( (vgicLR \<circ> vcpuVGIC $ vcpu)  aLU  [(index, virq)]);
+             setObject vcpuPtr $ vcpu \<lparr> vcpuVGIC := (vcpuVGIC vcpu) \<lparr> vgicLR := vcpuLR \<rparr>\<rparr>
+        od)
+        );
+    ct \<leftarrow> getCurThread;
+    setThreadState Restart ct
+od)"
+
+definition
+performARMVCPUInvocation :: "vcpuinvocation \<Rightarrow> unit kernel"
+where
+"performARMVCPUInvocation x0\<equiv> (case x0 of
+    (VCPUSetTCB vcpuPtr tcbPtr) \<Rightarrow>   
+    associateVCPUTCB vcpuPtr tcbPtr
+  | (VCPUReadRegister vcpuPtr reg) \<Rightarrow>   
+    invokeVCPUReadReg vcpuPtr reg
+  | (VCPUWriteRegister vcpuPtr reg val) \<Rightarrow>   
+    invokeVCPUWriteReg vcpuPtr reg val
+  | (VCPUInjectIRQ vcpuPtr index virq) \<Rightarrow>   
+    invokeVCPUInjectIRQ vcpuPtr index virq
+  )"
+
+definition
+decodeARMVCPUInvocation :: "machine_word \<Rightarrow> machine_word list \<Rightarrow> cptr \<Rightarrow> machine_word \<Rightarrow> arch_capability \<Rightarrow> (capability * machine_word) list \<Rightarrow> ( syscall_error , Arch.invocation ) kernel_f"
+where
+"decodeARMVCPUInvocation label args capIndex slot x4 extraCaps\<equiv> (let cap = x4 in
+  if isVCPUCap cap then  
+    (case invocationType label of
+          ArchInvocationLabel ARMVCPUSetTCB \<Rightarrow>  
+            decodeVCPUSetTCB cap extraCaps
+        | ArchInvocationLabel ARMVCPUReadReg \<Rightarrow>  
+            decodeVCPUReadReg args cap
+        | ArchInvocationLabel ARMVCPUWriteReg \<Rightarrow>  
+            decodeVCPUWriteReg args cap
+        | ArchInvocationLabel ARMVCPUInjectIRQ \<Rightarrow>  
+            decodeVCPUInjectIRQ args cap
+        | _ \<Rightarrow>   throw IllegalOperation
+        )
+  else   throw IllegalOperation
+  )"
+
+definition
+vcpuFinalise :: "machine_word \<Rightarrow> unit kernel"
+where
+"vcpuFinalise vcpuPtr\<equiv> (do
+    vcpu \<leftarrow> getObject vcpuPtr;
+    (case vcpuTCBPtr vcpu of
+          Some tcbPtr \<Rightarrow>   dissociateVCPUTCB vcpuPtr tcbPtr
+        | None \<Rightarrow>   return ()
+        );
+    hsCurVCPU \<leftarrow> gets (armHSCurVCPU \<circ> ksArchState);
+    (case hsCurVCPU of
+          Some (vcpuPtr, _) \<Rightarrow>   vcpuInvalidateActive
+        | _ \<Rightarrow>   return ()
+        )
+od)"
+
+
+
+end
+end
